impl_zero_copy_unit, always_false, copyful_pure_as_zero_copy

src/cddl/pulse/CDDL.Pulse.Parse.Base.fst
@@ -79,6 +79,33 @@ fn impl_copyful_unit
 
 inline_for_extraction noextract [@@noextract_to "krml"]
 ```pulse
+fn impl_zero_copy_unit
+    (#ty: Type0)
+    (vmatch: perm -> ty -> cbor -> slprop)
+    (#t: Ghost.erased typ)
+    (#tgt_serializable: Ghost.erased (unit -> bool))
+    (ps: Ghost.erased (parser_spec t unit tgt_serializable))
+: impl_zero_copy_parse #ty vmatch #(Ghost.reveal t) #unit #(Ghost.reveal tgt_serializable) (Ghost.reveal ps) #unit rel_unit // FIXME: WHY WHY WHY do I need to fill in all implicits by hand?
+=
+    (c: _)
+    (#p: _)
+    (#v: _)
+{
+  let res = ();
+  fold (rel_unit res ());
+  ghost fn aux (_: unit)
+  requires vmatch p c v ** rel_unit res ()
+  ensures vmatch p c v
+  {
+    unfold (rel_unit res ())
+  };
+  Trade.intro_trade _ _ _ aux;
+  res
+}
+```
+
+inline_for_extraction noextract [@@noextract_to "krml"]
+```pulse
 fn impl_copyful_always_false
     (#ty: Type0)
     (vmatch: perm -> ty -> cbor -> slprop)
@@ -93,6 +120,56 @@ fn impl_copyful_always_false
 {
   let res : squash False = Ghost.reveal ps v;
   fold (rel_always_false _ _ res res);
+  res
+}
+```
+
+inline_for_extraction noextract [@@noextract_to "krml"]
+```pulse
+fn impl_zero_copy_always_false
+    (#ty: Type0)
+    (vmatch: perm -> ty -> cbor -> slprop)
+    (#t: Ghost.erased typ)
+    (#tgt_serializable: Ghost.erased (squash False -> bool))
+    (ps: Ghost.erased (parser_spec t (squash False) tgt_serializable))
+: impl_zero_copy_parse #ty vmatch #(Ghost.reveal t) #(squash False) #(Ghost.reveal tgt_serializable) (Ghost.reveal ps) #(squash False) (rel_always_false (squash False) (squash False)) // FIXME: WHY WHY WHY do I need to fill in all implicits by hand?
+=
+    (c: _)
+    (#p: _)
+    (#v: _)
+{
+  let res : squash False = Ghost.reveal ps v;
+  fold (rel_always_false _ _ res res);
+  rewrite (vmatch p c v) as (Trade.trade (rel_always_false _ _ res res) (vmatch p c v)); // by contradiction
+  res
+}
+```
+
+inline_for_extraction noextract [@@noextract_to "krml"]
+```pulse
+fn impl_copyful_pure_as_zero_copy
+    (#ty: Type0)
+    (#vmatch: perm -> ty -> cbor -> slprop)
+    (#t: Ghost.erased typ)
+    (#tgt: Type0)
+    (#tgt_serializable: Ghost.erased (tgt -> bool))
+    (#ps: Ghost.erased (parser_spec t tgt tgt_serializable))
+    (i: impl_copyful_parse vmatch ps (rel_pure tgt))
+: impl_zero_copy_parse #_ vmatch #(Ghost.reveal t) #tgt #(Ghost.reveal tgt_serializable) (Ghost.reveal ps) #tgt (rel_pure tgt) 
+=
+    (c: ty)
+    (#p: perm)
+    (#v: Ghost.erased cbor)
+{
+  let res = i c;
+  with v' . assert (rel_pure tgt res v');
+  ghost fn aux (_: unit)
+  requires vmatch p c v ** rel_pure tgt res v'
+  ensures vmatch p c v
+  {
+    unfold (rel_pure tgt res v')
+  };
+  Trade.intro_trade _ _ _ aux;
   res
 }
 ```
